updated top

src/Framework/ANF0.v
@@ -534,6 +534,42 @@ Proof.
   inv H0; auto.
 Qed.
 
+Fixpoint occurs_free_case (cl : list (ctor_tag * exp)) : vars :=
+  match cl with
+  | [] => (Empty_set _)
+  | ((c, e) :: cl) => (occurs_free e) :|: (occurs_free_case cl)
+  end.
+
+Lemma occurs_free_case_compat cl :
+  forall y x,
+    (y \in (occurs_free_case cl)) ->
+    (y \in (occurs_free (Ecase x cl))).
+Proof.
+  unfold Ensembles.In.
+  induction cl; simpl; intros; auto.
+  - inv H.
+  - destruct a.
+    inv H; auto.
+Qed.
+
+Lemma occurs_free_case_inv cl :
+  forall y x,
+    (y \in (occurs_free (Ecase x cl))) ->
+    (y = x \/ (y \in (occurs_free_case cl))).
+Proof.
+  unfold Ensembles.In.
+  induction cl; simpl; intros; auto.
+  - inv H.
+    left; auto.
+  - destruct a.
+    inv H; auto.
+    + right; left; auto.
+    + eapply IHcl in H5; eauto; inv H5.
+      * left; auto.
+      * right; right; auto.
+Qed.
+
+(* Linking *)
 Definition link f x e1 e2 : exp :=
   Efun f [] e1
     (Eletapp x f [] e2).
